
\medskip

\begin{enumerate}
\item $E = x \times 2x + x \times 3 - 2 \times 2x - 2 \times 3 - 3x + 6$

$E = 2x^2 + 3x - 4x - 6 - 3x + 6$

$E = 2x^2 - 4x$.
\item $(x - 2)$ est un facteur commun de la diff√©rence, donc

$E = (x - 2)[(2x + 3) - 3]$

$E = (x - 2 )[2x + 3 - 3]$

$E = (x - 2)\times 2x = 2x(x - 2) = 2F$.
\item $(x - 2)(2x + 3) - 3(x - 2) = 0$  si et seulement si $2x(x - 2) = 0$ soit

$\left\{\begin{array}{l c l}
2x 		&=& 0 \quad \text{ou}\\
x - 2 	&=& 0
\end{array}\right.$ soit $\left\{\begin{array}{l c l}
x &=& 0 \quad\text{ou}\\
x &=&2
\end{array}\right.$

Les solutions sont $0$ et $2$.
\end{enumerate}

\vspace{0,5cm}

